libcrux-ml-kem/src/vector/avx2/serialize.rs
@@ -102,113 +102,101 @@ assert (forall (i: nat {i < 16}). bv i == ${vector} (i * 16)) by (
 }
 
 #[inline(always)]
-pub(crate) fn deserialize_1(bytes: &[u8]) -> Vec256 {
-    // We need to take each bit from the 2 bytes of input and put them
-    // into their own 16-bit lane. Ideally, we'd load the two bytes into the vector,
-    // duplicate them, and right-shift the 0th element by 0 bits,
-    // the first element by 1 bit, the second by 2 bits and so on before AND-ing
-    // with 0x1 to leave only the least signifinicant bit.
-    // But since |_mm256_srlv_epi16| does not exist, so we have to resort to a
-    // workaround.
-    //
-    // Rather than shifting each element by a different amount, we'll multiply
-    // each element by a value such that the bit we're interested in becomes the most
-    // significant bit.
-
-    // The coefficients are loaded as follows:
-    let coefficients = mm256_set_epi16(
-        bytes[1] as i16,
-        bytes[1] as i16,
-        bytes[1] as i16,
-        bytes[1] as i16,
-        bytes[1] as i16,
-        bytes[1] as i16,
-        bytes[1] as i16,
-        bytes[1] as i16,
-        bytes[0] as i16,
-        bytes[0] as i16,
-        bytes[0] as i16,
-        bytes[0] as i16,
-        bytes[0] as i16,
-        bytes[0] as i16,
-        bytes[0] as i16,
-        bytes[0] as i16,
-    );
-
-    // And this vector, when multiplied with the previous one, ensures that the
-    // bit we'd like to keep in each lane becomes the most significant bit upon
-    // multiplication.
-    let coefficients_in_msb = mm256_mullo_epi16(
-        coefficients,
-        mm256_set_epi16(
-            1 << 8,
-            1 << 9,
-            1 << 10,
-            1 << 11,
-            1 << 12,
-            1 << 13,
-            1 << 14,
-            -32768,
-            1 << 8,
-            1 << 9,
-            1 << 10,
-            1 << 11,
-            1 << 12,
-            1 << 13,
-            1 << 14,
-            -32768,
-        ),
-    );
-
-    // Now that they're all in the most significant bit position, shift them
-    // down to the least significant bit.
-    let result = mm256_srli_epi16::<15>(coefficients_in_msb);
-
-    hax_lib::fstar!(
-        r#"
-let bv = bit_vec_of_int_t_array (${bytes} <: t_Array _ (sz 2)) 8 in
-assert (forall (i: nat {i < 256}). (if i % 16 = 0 then bv i else 0) == result i) by (
-  let open FStar.Tactics in
-  let open Tactics.Utils in
-  let light_norm () =
-    // simplify the term: compute `+/*+` on ints, remove cast/array_of_list/funext indirections
-    norm [ iota; primops
-         ; delta_namespace [
-           `%cast; `%cast_tc_integers
-             ; `%bit_vec_of_int_t_array
-             ; `%Rust_primitives.Hax.array_of_list
-             ; "FStar.FunctionalExtensionality"
-             ; `%bits;`%Lib.IntTypes.bits
-           ]
-    ] in
-  light_norm ();
-  // instantiate the forall with concrete values, and run a tactic for each possible values
-  prove_forall_nat_pointwise (print_time "SMT query succeeded in " (fun _ ->
-    light_norm ();
-    // norm index rewrites `Seq.index (Seq.seq_of_list ...) N` or
-    // `List.Tot.index ... N` when we have list literals
-    Tactics.Seq.norm_index ();
-    // Reduce more aggressively
-    norm [iota; primops; zeta_full;
-          delta_namespace [
-            "FStar";
-            "BitVec";
-          ]; unascribe
-          ];
-    // Rewrite and normalize machine integers, hopefully in ints
-    Tactics.MachineInts.(transform norm_machine_int_term);
-    // norm: primops to get rid of >=, <=, +, *, -, etc.
-    //       zeta delta iota: normalize bitvectors
-    norm [iota; primops; zeta; delta];
-    dump' "Goal:";
-    // ask the smt to solve now
-    smt_sync ()
-  ))
-)
+#[hax_lib::requires(bytes.len() == 2)]
+#[hax_lib::ensures(|coefficients| fstar!(
+        r#"forall (i:nat{i < 256}).
+      $coefficients i
+    = ( if i % 16 >= 1 then 0
+        else let j = (i / 16) * 1 + i % 16 in
+             bit_vec_of_int_t_array ($bytes <: t_Array _ (sz 2)) 8 j))
 "#
-    );
+))]
+#[hax_lib::fstar::before("#restart-solver")]
+pub(crate) fn deserialize_1(bytes: &[u8]) -> Vec256 {
+    #[hax_lib::ensures(|coefficients| fstar!(
+        r#"forall (i:nat{i < 256}).
+      $coefficients i
+    = ( if i % 16 >= 1 then 0
+        else let j = (i / 16) * 1 + i % 16 in
+             if i < 128 then get_bit $a (sz j) else get_bit $b (sz (j - 8)))
+"#
+    ))]
+    #[hax_lib::fstar::before(r#"[@@"opaque_to_smt"]"#)]
+    #[inline(always)]
+    pub(crate) fn deserialize_1_u8s(a: u8, b: u8) -> Vec256 {
+        deserialize_1_i16s(a as i16, b as i16)
+    }
 
-    result
+    #[hax_lib::ensures(|coefficients| fstar!(
+        r#"forall (i:nat{i < 256}).
+      $coefficients i
+    = ( if i % 16 >= 1 then 0
+        else let j = (i / 16) * 1 + i % 16 in
+             if i < 128 then get_bit $a (sz j) else get_bit $b (sz (j - 8)))
+"#
+    ))]
+    #[inline(always)]
+    #[hax_lib::fstar::before(r#"[@@"opaque_to_smt"]"#)]
+    pub(crate) fn deserialize_1_i16s(a: i16, b: i16) -> Vec256 {
+        // We need to take each bit from the 2 bytes of input and put them
+        // into their own 16-bit lane. Ideally, we'd load the two bytes into the vector,
+        // duplicate them, and right-shift the 0th element by 0 bits,
+        // the first element by 1 bit, the second by 2 bits and so on before AND-ing
+        // with 0x1 to leave only the least signifinicant bit.
+        // But since |_mm256_srlv_epi16| does not exist, so we have to resort to a
+        // workaround.
+        //
+        // Rather than shifting each element by a different amount, we'll multiply
+        // each element by a value such that the bit we're interested in becomes the most
+        // significant bit.
+        // The coefficients are loaded as follows:
+        let coefficients = mm256_set_epi16(b, b, b, b, b, b, b, b, a, a, a, a, a, a, a, a);
+
+        // And this vector, when multiplied with the previous one, ensures that the
+        // bit we'd like to keep in each lane becomes the most significant bit upon
+        // multiplication.
+        let coefficients_in_msb = mm256_mullo_epi16(
+            coefficients,
+            mm256_set_epi16(
+                1 << 8,
+                1 << 9,
+                1 << 10,
+                1 << 11,
+                1 << 12,
+                1 << 13,
+                1 << 14,
+                -32768,
+                1 << 8,
+                1 << 9,
+                1 << 10,
+                1 << 11,
+                1 << 12,
+                1 << 13,
+                1 << 14,
+                -32768,
+            ),
+        );
+
+        // Now that they're all in the most significant bit position, shift them
+        // down to the least significant bit.
+        mm256_srli_epi16::<15>(coefficients_in_msb)
+    }
+
+    deserialize_1_u8s(bytes[0], bytes[1])
+}
+
+/// `mm256_concat_pairs_n(n, x)` is then a sequence of 32 bits packets
+/// of the shape `0b0…0b₁…bₙa₁…aₙ`, if `x` is a sequence of pairs of
+/// 16 bits, of the shape `(0b0…0a₁…aₙ, 0b0…0b₁…bₙ)` (where the last
+/// `n` bits are non-zero).
+#[hax_lib::fstar::replace(interface, "include BitVec.Intrinsics {mm256_concat_pairs_n}")]
+#[inline(always)]
+fn mm256_concat_pairs_n(n: u8, x: Vec256) -> Vec256 {
+    let n = 1 << n;
+    mm256_madd_epi16(
+        x,
+        mm256_set_epi16(n, 1, n, 1, n, 1, n, 1, n, 1, n, 1, n, 1, n, 1),
+    )
 }
 
 #[hax_lib::requires(
@@ -318,112 +306,119 @@ assert (forall (i: nat {i < 64}).
     serialized[0..8].try_into().unwrap()
 }
 
-#[hax_lib::requires(bytes.len() == 8)]
 #[inline(always)]
+#[hax_lib::requires(bytes.len() == 8)]
+#[hax_lib::ensures(|result| fstar!(r#"forall (i: nat{i < 256}).
+  $result i = (if i % 16 >= 4 then 0
+               else let j = (i / 16) * 4 + i % 16 in
+                     bit_vec_of_int_t_array ($bytes <: t_Array _ (sz 8)) 8 j)"#))]
+#[hax_lib::fstar::before("#restart-solver")]
 pub(crate) fn deserialize_4(bytes: &[u8]) -> Vec256 {
-    // Every 4 bits from each byte of input should be put into its own 16-bit lane.
-    // Since |_mm256_srlv_epi16| does not exist, we have to resort to a workaround.
-    //
-    // Rather than shifting each element by a different amount, we'll multiply
-    // each element by a value such that the bits we're interested in become the most
-    // significant bits (of an 8-bit value).
-    let coefficients = mm256_set_epi16(
-        // In this lane, the 4 bits we need to put are already the most
-        // significant bits of |bytes[7]|.
-        bytes[7] as i16,
-        // In this lane, the 4 bits we need to put are the least significant bits,
-        // so we need to shift the 4 least-significant bits of |bytes[7]| to the
-        // most significant bits (of an 8-bit value).
-        bytes[7] as i16,
-        // and so on ...
-        bytes[6] as i16,
-        bytes[6] as i16,
-        bytes[5] as i16,
-        bytes[5] as i16,
-        bytes[4] as i16,
-        bytes[4] as i16,
-        bytes[3] as i16,
-        bytes[3] as i16,
-        bytes[2] as i16,
-        bytes[2] as i16,
-        bytes[1] as i16,
-        bytes[1] as i16,
-        bytes[0] as i16,
-        bytes[0] as i16,
-    );
-
-    let coefficients_in_msb = mm256_mullo_epi16(
-        coefficients,
-        mm256_set_epi16(
-            // These constants are chosen to shift the bits of the values
-            // that we loaded into |coefficients|.
-            1 << 0,
-            1 << 4,
-            1 << 0,
-            1 << 4,
-            1 << 0,
-            1 << 4,
-            1 << 0,
-            1 << 4,
-            1 << 0,
-            1 << 4,
-            1 << 0,
-            1 << 4,
-            1 << 0,
-            1 << 4,
-            1 << 0,
-            1 << 4,
-        ),
-    );
-
-    // Once the 4-bit coefficients are in the most significant positions (of
-    // an 8-bit value), shift them all down by 4.
-    let coefficients_in_lsb = mm256_srli_epi16::<4>(coefficients_in_msb);
-
-    // Zero the remaining bits.
-    let result = mm256_and_si256(coefficients_in_lsb, mm256_set1_epi16((1 << 4) - 1));
-
-    hax_lib::fstar!(
-        r#"
-let bv = bit_vec_of_int_t_array (${bytes} <: t_Array _ (sz 8)) 8 in  
-assert (forall (i: nat {i < 64}). bv i == ${result} ((i / 4) * 16 + i % 4)) by (
-  let open FStar.Tactics in
-  let open Tactics.Utils in
-  let light_norm () = 
-    norm [ iota; primops
-         ; delta_namespace [
-           `%cast; `%cast_tc_integers
-             ; `%bit_vec_of_int_t_array
-             ; `%Rust_primitives.Hax.array_of_list
-             ; "FStar.FunctionalExtensionality"
-             ; `%bits;`%Lib.IntTypes.bits
-           ]
-    ] in
-  light_norm ();
-  prove_forall_nat_pointwise (print_time "SMT query succeeded in " (fun _ ->
-    light_norm ();
-    Tactics.Seq.norm_index ();
-    norm [iota; primops; zeta_full;
-          delta_namespace [
-            "FStar";
-            "BitVec";
-          ]; unascribe
-          ];
-    Tactics.MachineInts.(transform norm_machine_int_term);
-    norm [iota; primops; zeta_full;
-          delta_namespace [
-            "FStar";
-            "BitVec";
-          ]; unascribe
-          ];
-    dump' "Goal:";
-    smt_sync ()
-  ))
-)
+    #[hax_lib::ensures(|coefficients| fstar!(
+        r#"forall (i:nat{i < 256}).
+      $coefficients i
+    = ( if i % 16 < 4
+        then let j = (i / 16) * 4 + i % 16 in
+             (match i / 32 with
+             | 0 -> get_bit $b0 (sz j)
+             | 1 -> get_bit $b1 (sz (j - 8))
+             | 2 -> get_bit $b2 (sz (j - 16))
+             | 3 -> get_bit $b3 (sz (j - 24))
+             | 4 -> get_bit $b4 (sz (j - 32))
+             | 5 -> get_bit $b5 (sz (j - 40))
+             | 6 -> get_bit $b6 (sz (j - 48))
+             | 7 -> get_bit $b7 (sz (j - 56)))
+        else 0)
 "#
-    );
+    ))]
+    #[inline(always)]
+    #[hax_lib::fstar::before(r#"[@@"opaque_to_smt"]"#)]
+    fn deserialize_4_u8s(b0: u8, b1: u8, b2: u8, b3: u8, b4: u8, b5: u8, b6: u8, b7: u8) -> Vec256 {
+        deserialize_4_i16s(
+            b0 as i16, b1 as i16, b2 as i16, b3 as i16, b4 as i16, b5 as i16, b6 as i16, b7 as i16,
+        )
+    }
 
-    result
+    #[hax_lib::ensures(|coefficients| fstar!(
+        r#"forall (i:nat{i < 256}).
+      $coefficients i
+    = ( if i % 16 < 4
+        then let j = (i / 16) * 4 + i % 16 in
+             (match i / 32 with
+             | 0 -> get_bit $b0 (sz j)
+             | 1 -> get_bit $b1 (sz (j - 8))
+             | 2 -> get_bit $b2 (sz (j - 16))
+             | 3 -> get_bit $b3 (sz (j - 24))
+             | 4 -> get_bit $b4 (sz (j - 32))
+             | 5 -> get_bit $b5 (sz (j - 40))
+             | 6 -> get_bit $b6 (sz (j - 48))
+             | 7 -> get_bit $b7 (sz (j - 56)))
+        else 0)
+"#
+    ))]
+    #[inline(always)]
+    #[hax_lib::fstar::before(r#"[@@"opaque_to_smt"]"#)]
+    fn deserialize_4_i16s(
+        b0: i16,
+        b1: i16,
+        b2: i16,
+        b3: i16,
+        b4: i16,
+        b5: i16,
+        b6: i16,
+        b7: i16,
+    ) -> Vec256 {
+        // Every 4 bits from each byte of input should be put into its own 16-bit lane.
+        // Since |_mm256_srlv_epi16| does not exist, we have to resort to a workaround.
+        //
+        // Rather than shifting each element by a different amount, we'll multiply
+        // each element by a value such that the bits we're interested in become the most
+        // significant bits (of an 8-bit value).
+        let coefficients = mm256_set_epi16(
+            // In this lane, the 4 bits we need to put are already the most
+            // significant bits of |bytes[7]| (that is, b7).
+            b7,
+            // In this lane, the 4 bits we need to put are the least significant bits,
+            // so we need to shift the 4 least-significant bits of |b7| to the
+            // most significant bits (of an 8-bit value).
+            b7, // and so on ...
+            b6, b6, b5, b5, b4, b4, b3, b3, b2, b2, b1, b1, b0, b0,
+        );
+        let coefficients_in_msb = mm256_mullo_epi16(
+            coefficients,
+            mm256_set_epi16(
+                // These constants are chosen to shift the bits of the values
+                // that we loaded into |coefficients|.
+                1 << 0,
+                1 << 4,
+                1 << 0,
+                1 << 4,
+                1 << 0,
+                1 << 4,
+                1 << 0,
+                1 << 4,
+                1 << 0,
+                1 << 4,
+                1 << 0,
+                1 << 4,
+                1 << 0,
+                1 << 4,
+                1 << 0,
+                1 << 4,
+            ),
+        );
+
+        // Once the 4-bit coefficients are in the most significant positions (of
+        // an 8-bit value), shift them all down by 4.
+        let coefficients_in_lsb = mm256_srli_epi16::<4>(coefficients_in_msb);
+
+        // Zero the remaining bits.
+        mm256_and_si256(coefficients_in_lsb, mm256_set1_epi16((1 << 4) - 1))
+    }
+
+    deserialize_4_u8s(
+        bytes[0], bytes[1], bytes[2], bytes[3], bytes[4], bytes[5], bytes[6], bytes[7],
+    )
 }
 
 #[inline(always)]
@@ -523,6 +518,22 @@ pub(crate) fn serialize_5(vector: Vec256) -> [u8; 10] {
     serialized[0..10].try_into().unwrap()
 }
 
+/// We cannot model `mm256_inserti128_si256` on its own: it produces a
+/// Vec256 where the upper 128 bits are undefined. Thus
+/// `mm256_inserti128_si256` is not pure.
+///
+/// Luckily, we always call `mm256_castsi128_si256` right after
+/// `mm256_inserti128_si256`: this composition sets the upper bits,
+/// making the whole computation pure again.
+#[inline(always)]
+#[hax_lib::fstar::replace(
+    interface,
+    "include BitVec.Intrinsics {mm256_si256_from_two_si128 as ${mm256_si256_from_two_si128}}"
+)]
+fn mm256_si256_from_two_si128(lower: Vec128, upper: Vec128) -> Vec256 {
+    mm256_inserti128_si256::<1>(mm256_castsi128_si256(lower), upper)
+}
+
 #[inline(always)]
 pub(crate) fn deserialize_5(bytes: &[u8]) -> Vec256 {
     let coefficients = mm_set_epi8(
@@ -530,8 +541,7 @@ pub(crate) fn deserialize_5(bytes: &[u8]) -> Vec256 {
         bytes[3], bytes[3], bytes[2], bytes[2], bytes[1], bytes[1], bytes[0],
     );
 
-    let coefficients_loaded = mm256_castsi128_si256(coefficients);
-    let coefficients_loaded = mm256_inserti128_si256::<1>(coefficients_loaded, coefficients);
+    let coefficients_loaded = mm256_si256_from_two_si128(coefficients, coefficients);
 
     let coefficients = mm256_shuffle_epi8(
         coefficients_loaded,
@@ -566,6 +576,8 @@ pub(crate) fn deserialize_5(bytes: &[u8]) -> Vec256 {
 }
 
 #[inline(always)]
+#[hax_lib::requires(fstar!("forall (i: nat{i < 256}). i % 16 < 10 || vector i = 0"))]
+#[hax_lib::ensures(|r| fstar!("forall (i: nat{i < 160}). bit_vec_of_int_t_array r 8 i == vector ((i/10) * 16 + i%10)"))]
 pub(crate) fn serialize_10(vector: Vec256) -> [u8; 20] {
     let mut serialized = [0u8; 32];
 
@@ -582,27 +594,7 @@ pub(crate) fn serialize_10(vector: Vec256) -> [u8; 20] {
     // 0¹²b₉b₈b₇b₆b₅b₄b₃b₂b₁b₀a₉a₈a₇a₆a₅a₄a₃a₂a₁a₀ 0¹²d₉d₈d₇d₆d₅d₄d₃d₂d₁d₀c₉c₈c₇c₆c₅c₄c₃c₂c₁c₀ | ↩
     // 0¹²f₉f₈f₇f₆f₅f₄f₃f₂f₁f₀e₉e₈e₇e₆e₅e₄e₃e₂e₁e₀ 0¹²h₉h₈h₇h₆h₅h₄h₃h₂h₁h₀g₉g₈g₇g₆g₅g₄g₃g₂g₁g₀ | ↩
     // ....
-    let adjacent_2_combined = mm256_madd_epi16(
-        vector,
-        mm256_set_epi16(
-            1 << 10,
-            1,
-            1 << 10,
-            1,
-            1 << 10,
-            1,
-            1 << 10,
-            1,
-            1 << 10,
-            1,
-            1 << 10,
-            1,
-            1 << 10,
-            1,
-            1 << 10,
-            1,
-        ),
-    );
+    let adjacent_2_combined = mm256_concat_pairs_n(10, vector);
 
     // Shifting up the values at the even indices by 12, we get:
     //
@@ -649,51 +641,90 @@ pub(crate) fn serialize_10(vector: Vec256) -> [u8; 20] {
 
     // and 64 bits starting at position 0 in the upper 128-bit lane.
     let upper_8 = mm256_extracti128_si256::<1>(adjacent_8_combined);
+    hax_lib::fstar!(
+        r#"
+      assert_norm (
+         BitVec.Utils.forall_n 80 (fun i -> lower_8_ i = vector (      (i/10) * 16 + i%10))
+      && BitVec.Utils.forall_n 80 (fun i -> upper_8_ i = vector (128 + (i/10) * 16 + i%10))
+      )
+    "#
+    );
     mm_storeu_bytes_si128(&mut serialized[10..26], upper_8);
 
     serialized[0..20].try_into().unwrap()
 }
 
 #[inline(always)]
+#[hax_lib::requires(fstar!(r#"Seq.length bytes == 20"#))]
+#[hax_lib::ensures(|result| fstar!(r#"forall (i: nat{i < 256}).
+  $result i = (if i % 16 >= 10 then 0
+               else let j = (i / 16) * 10 + i % 16 in
+                     bit_vec_of_int_t_array ($bytes <: t_Array _ (sz 20)) 8 j)"#))]
 pub(crate) fn deserialize_10(bytes: &[u8]) -> Vec256 {
-    let shift_lsbs_to_msbs = mm256_set_epi16(
-        1 << 0,
-        1 << 2,
-        1 << 4,
-        1 << 6,
-        1 << 0,
-        1 << 2,
-        1 << 4,
-        1 << 6,
-        1 << 0,
-        1 << 2,
-        1 << 4,
-        1 << 6,
-        1 << 0,
-        1 << 2,
-        1 << 4,
-        1 << 6,
-    );
+    #[inline(always)]
+    #[hax_lib::ensures(|coefficients| fstar!(r#"
+forall (i: nat {i < 256}).
+      $coefficients i
+    = ( if i % 16 >= 10 then 0
+        else let j = (i / 16) * 10 + i % 16 in
+             if i < 128 then $lower_coefficients0 j else $upper_coefficients0 (j - 32)))
+"#))]
+    #[hax_lib::fstar::before(r#"[@@"opaque_to_smt"]"#)]
+    fn deserialize_10_vec(lower_coefficients0: Vec128, upper_coefficients0: Vec128) -> Vec256 {
+        let lower_coefficients = mm_shuffle_epi8(
+            lower_coefficients0,
+            mm_set_epi8(9, 8, 8, 7, 7, 6, 6, 5, 4, 3, 3, 2, 2, 1, 1, 0),
+        );
+        let upper_coefficients = mm_shuffle_epi8(
+            upper_coefficients0,
+            mm_set_epi8(15, 14, 14, 13, 13, 12, 12, 11, 10, 9, 9, 8, 8, 7, 7, 6),
+        );
 
-    let lower_coefficients = mm_loadu_si128(&bytes[0..16]);
-    let lower_coefficients = mm_shuffle_epi8(
-        lower_coefficients,
-        mm_set_epi8(9, 8, 8, 7, 7, 6, 6, 5, 4, 3, 3, 2, 2, 1, 1, 0),
-    );
-    let upper_coefficients = mm_loadu_si128(&bytes[4..20]);
-    let upper_coefficients = mm_shuffle_epi8(
-        upper_coefficients,
-        mm_set_epi8(15, 14, 14, 13, 13, 12, 12, 11, 10, 9, 9, 8, 8, 7, 7, 6),
-    );
+        let coefficients = mm256_si256_from_two_si128(lower_coefficients, upper_coefficients);
 
-    let coefficients = mm256_castsi128_si256(lower_coefficients);
-    let coefficients = mm256_inserti128_si256::<1>(coefficients, upper_coefficients);
+        let coefficients = mm256_mullo_epi16(
+            coefficients,
+            mm256_set_epi16(
+                1 << 0,
+                1 << 2,
+                1 << 4,
+                1 << 6,
+                1 << 0,
+                1 << 2,
+                1 << 4,
+                1 << 6,
+                1 << 0,
+                1 << 2,
+                1 << 4,
+                1 << 6,
+                1 << 0,
+                1 << 2,
+                1 << 4,
+                1 << 6,
+            ),
+        );
+        let coefficients = mm256_srli_epi16::<6>(coefficients);
+        // Here I can prove this `and` is not useful
+        let coefficients = mm256_and_si256(coefficients, mm256_set1_epi16((1 << 10) - 1));
+        hax_lib::fstar!(
+            r#"
+assert_norm(BitVec.Utils.forall256 (fun i -> 
+      $coefficients i
+    = ( if i % 16 < 10
+        then let j = (i / 16) * 10 + i % 16 in
+             if i < 128 then $lower_coefficients0 j else $upper_coefficients0 (j - 32)
+        else 0)))
+"#
+        );
+        coefficients
+    }
 
-    let coefficients = mm256_mullo_epi16(coefficients, shift_lsbs_to_msbs);
-    let coefficients = mm256_srli_epi16::<6>(coefficients);
-    let coefficients = mm256_and_si256(coefficients, mm256_set1_epi16((1 << 10) - 1));
-
-    coefficients
+    let lower_coefficients = &bytes[0..16];
+    let upper_coefficients = &bytes[4..20];
+    deserialize_10_vec(
+        mm_loadu_si128(lower_coefficients),
+        mm_loadu_si128(upper_coefficients),
+    )
 }
 
 #[inline(always)]
@@ -759,43 +790,69 @@ pub(crate) fn serialize_12(vector: Vec256) -> [u8; 24] {
 }
 
 #[inline(always)]
+#[hax_lib::requires(fstar!(r#"Seq.length bytes == 24"#))]
+#[hax_lib::ensures(|result| fstar!(r#"forall (i: nat{i < 256}).
+  $result i = (if i % 16 >= 12 then 0
+               else let j = (i / 16) * 12 + i % 16 in
+                     bit_vec_of_int_t_array ($bytes <: t_Array _ (sz 24)) 8 j)"#))]
 pub(crate) fn deserialize_12(bytes: &[u8]) -> Vec256 {
-    let shift_lsbs_to_msbs = mm256_set_epi16(
-        1 << 0,
-        1 << 4,
-        1 << 0,
-        1 << 4,
-        1 << 0,
-        1 << 4,
-        1 << 0,
-        1 << 4,
-        1 << 0,
-        1 << 4,
-        1 << 0,
-        1 << 4,
-        1 << 0,
-        1 << 4,
-        1 << 0,
-        1 << 4,
-    );
+    #[inline(always)]
+    #[hax_lib::ensures(|coefficients| fstar!(r#"
+forall (i: nat {i < 256}).
+      $coefficients i
+    = ( if i % 16 >= 12 then 0
+        else let j = (i / 16) * 12 + i % 16 in
+             if i < 128 then $lower_coefficients0 j else $upper_coefficients0 (j - 64)))
+"#))]
+    #[hax_lib::fstar::before(r#"[@@"opaque_to_smt"]"#)]
+    fn deserialize_12_vec(lower_coefficients0: Vec128, upper_coefficients0: Vec128) -> Vec256 {
+        let lower_coefficients = mm_shuffle_epi8(
+            lower_coefficients0,
+            mm_set_epi8(11, 10, 10, 9, 8, 7, 7, 6, 5, 4, 4, 3, 2, 1, 1, 0),
+        );
+        let upper_coefficients = mm_shuffle_epi8(
+            upper_coefficients0,
+            mm_set_epi8(15, 14, 14, 13, 12, 11, 11, 10, 9, 8, 8, 7, 6, 5, 5, 4),
+        );
 
+        let coefficients = mm256_si256_from_two_si128(lower_coefficients, upper_coefficients);
+
+        let coefficients = mm256_mullo_epi16(
+            coefficients,
+            mm256_set_epi16(
+                1 << 0,
+                1 << 4,
+                1 << 0,
+                1 << 4,
+                1 << 0,
+                1 << 4,
+                1 << 0,
+                1 << 4,
+                1 << 0,
+                1 << 4,
+                1 << 0,
+                1 << 4,
+                1 << 0,
+                1 << 4,
+                1 << 0,
+                1 << 4,
+            ),
+        );
+        let coefficients = mm256_srli_epi16::<4>(coefficients);
+        let coefficients = mm256_and_si256(coefficients, mm256_set1_epi16((1 << 12) - 1));
+        hax_lib::fstar!(
+            r#"
+assert_norm(BitVec.Utils.forall256 (fun i -> 
+      $coefficients i
+    = ( if i % 16 < 12
+        then let j = (i / 16) * 12 + i % 16 in
+             if i < 128 then $lower_coefficients0 j else $upper_coefficients0 (j - 64)
+        else 0)))
+"#
+        );
+        coefficients
+    }
     let lower_coefficients = mm_loadu_si128(&bytes[0..16]);
-    let lower_coefficients = mm_shuffle_epi8(
-        lower_coefficients,
-        mm_set_epi8(11, 10, 10, 9, 8, 7, 7, 6, 5, 4, 4, 3, 2, 1, 1, 0),
-    );
     let upper_coefficients = mm_loadu_si128(&bytes[8..24]);
-    let upper_coefficients = mm_shuffle_epi8(
-        upper_coefficients,
-        mm_set_epi8(15, 14, 14, 13, 12, 11, 11, 10, 9, 8, 8, 7, 6, 5, 5, 4),
-    );
-
-    let coefficients = mm256_castsi128_si256(lower_coefficients);
-    let coefficients = mm256_inserti128_si256::<1>(coefficients, upper_coefficients);
-
-    let coefficients = mm256_mullo_epi16(coefficients, shift_lsbs_to_msbs);
-    let coefficients = mm256_srli_epi16::<4>(coefficients);
-    let coefficients = mm256_and_si256(coefficients, mm256_set1_epi16((1 << 12) - 1));
-
-    coefficients
+    deserialize_12_vec(lower_coefficients, upper_coefficients)
 }
