libcrux-ml-kem/proofs/fstar/extraction/Libcrux_ml_kem.Vector.Avx2.Serialize.fsti
@@ -9,28 +9,118 @@ let _ =
   let open Libcrux_ml_kem.Vector.Portable in
   ()
 
+val deserialize_1___deserialize_1_i16s (a b: i16)
+    : Prims.Pure Libcrux_intrinsics.Avx2_extract.t_Vec256
+      Prims.l_True
+      (ensures
+        fun coefficients ->
+          let coefficients:Libcrux_intrinsics.Avx2_extract.t_Vec256 = coefficients in
+          forall (i: nat{i < 256}).
+            coefficients i =
+            (if i % 16 >= 1
+              then 0
+              else
+                let j = (i / 16) * 1 + i % 16 in
+                if i < 128 then get_bit a (sz j) else get_bit b (sz (j - 8))))
+
+val deserialize_1___deserialize_1_u8s (a b: u8)
+    : Prims.Pure Libcrux_intrinsics.Avx2_extract.t_Vec256
+      Prims.l_True
+      (ensures
+        fun coefficients ->
+          let coefficients:Libcrux_intrinsics.Avx2_extract.t_Vec256 = coefficients in
+          forall (i: nat{i < 256}).
+            coefficients i =
+            (if i % 16 >= 1
+              then 0
+              else
+                let j = (i / 16) * 1 + i % 16 in
+                if i < 128 then get_bit a (sz j) else get_bit b (sz (j - 8))))
+
 val deserialize_1_ (bytes: t_Slice u8)
-    : Prims.Pure Libcrux_intrinsics.Avx2_extract.t_Vec256 Prims.l_True (fun _ -> Prims.l_True)
+    : Prims.Pure Libcrux_intrinsics.Avx2_extract.t_Vec256
+      (requires (Core.Slice.impl__len #u8 bytes <: usize) =. sz 2)
+      (ensures
+        fun coefficients ->
+          let coefficients:Libcrux_intrinsics.Avx2_extract.t_Vec256 = coefficients in
+          forall (i: nat{i < 256}).
+            coefficients i =
+            (if i % 16 >= 1
+              then 0
+              else
+                let j = (i / 16) * 1 + i % 16 in
+                bit_vec_of_int_t_array (bytes <: t_Array _ (sz 2)) 8 j))
 
-val deserialize_10_ (bytes: t_Slice u8)
-    : Prims.Pure Libcrux_intrinsics.Avx2_extract.t_Vec256 Prims.l_True (fun _ -> Prims.l_True)
+val deserialize_4___deserialize_4_i16s (b0 b1 b2 b3 b4 b5 b6 b7: i16)
+    : Prims.Pure Libcrux_intrinsics.Avx2_extract.t_Vec256
+      Prims.l_True
+      (ensures
+        fun coefficients ->
+          let coefficients:Libcrux_intrinsics.Avx2_extract.t_Vec256 = coefficients in
+          forall (i: nat{i < 256}).
+            coefficients i =
+            (if i % 16 < 4
+              then
+                let j = (i / 16) * 4 + i % 16 in
+                (match i / 32 with
+                  | 0 -> get_bit b0 (sz j)
+                  | 1 -> get_bit b1 (sz (j - 8))
+                  | 2 -> get_bit b2 (sz (j - 16))
+                  | 3 -> get_bit b3 (sz (j - 24))
+                  | 4 -> get_bit b4 (sz (j - 32))
+                  | 5 -> get_bit b5 (sz (j - 40))
+                  | 6 -> get_bit b6 (sz (j - 48))
+                  | 7 -> get_bit b7 (sz (j - 56)))
+              else 0))
 
-val deserialize_12_ (bytes: t_Slice u8)
-    : Prims.Pure Libcrux_intrinsics.Avx2_extract.t_Vec256 Prims.l_True (fun _ -> Prims.l_True)
+val deserialize_4___deserialize_4_u8s (b0 b1 b2 b3 b4 b5 b6 b7: u8)
+    : Prims.Pure Libcrux_intrinsics.Avx2_extract.t_Vec256
+      Prims.l_True
+      (ensures
+        fun coefficients ->
+          let coefficients:Libcrux_intrinsics.Avx2_extract.t_Vec256 = coefficients in
+          forall (i: nat{i < 256}).
+            coefficients i =
+            (if i % 16 < 4
+              then
+                let j = (i / 16) * 4 + i % 16 in
+                (match i / 32 with
+                  | 0 -> get_bit b0 (sz j)
+                  | 1 -> get_bit b1 (sz (j - 8))
+                  | 2 -> get_bit b2 (sz (j - 16))
+                  | 3 -> get_bit b3 (sz (j - 24))
+                  | 4 -> get_bit b4 (sz (j - 32))
+                  | 5 -> get_bit b5 (sz (j - 40))
+                  | 6 -> get_bit b6 (sz (j - 48))
+                  | 7 -> get_bit b7 (sz (j - 56)))
+              else 0))
 
 val deserialize_4_ (bytes: t_Slice u8)
     : Prims.Pure Libcrux_intrinsics.Avx2_extract.t_Vec256
       (requires (Core.Slice.impl__len #u8 bytes <: usize) =. sz 8)
-      (fun _ -> Prims.l_True)
+      (ensures
+        fun result ->
+          let result:Libcrux_intrinsics.Avx2_extract.t_Vec256 = result in
+          forall (i: nat{i < 256}).
+            result i =
+            (if i % 16 >= 4
+              then 0
+              else
+                let j = (i / 16) * 4 + i % 16 in
+                bit_vec_of_int_t_array (bytes <: t_Array _ (sz 8)) 8 j))
 
-val deserialize_5_ (bytes: t_Slice u8)
-    : Prims.Pure Libcrux_intrinsics.Avx2_extract.t_Vec256 Prims.l_True (fun _ -> Prims.l_True)
+include BitVec.Intrinsics {mm256_concat_pairs_n}
 
 val serialize_1_ (vector: Libcrux_intrinsics.Avx2_extract.t_Vec256)
     : Prims.Pure (t_Array u8 (sz 2)) Prims.l_True (fun _ -> Prims.l_True)
 
 val serialize_10_ (vector: Libcrux_intrinsics.Avx2_extract.t_Vec256)
-    : Prims.Pure (t_Array u8 (sz 20)) Prims.l_True (fun _ -> Prims.l_True)
+    : Prims.Pure (t_Array u8 (sz 20))
+      (requires forall (i: nat{i < 256}). i % 16 < 10 || vector i = 0)
+      (ensures
+        fun r ->
+          let r:t_Array u8 (sz 20) = r in
+          forall (i: nat{i < 160}). bit_vec_of_int_t_array r 8 i == vector ((i / 10) * 16 + i % 10))
 
 val serialize_12_ (vector: Libcrux_intrinsics.Avx2_extract.t_Vec256)
     : Prims.Pure (t_Array u8 (sz 24)) Prims.l_True (fun _ -> Prims.l_True)
@@ -42,6 +132,66 @@ val serialize_4_ (vector: Libcrux_intrinsics.Avx2_extract.t_Vec256)
     : Prims.Pure (t_Array u8 (sz 8))
       (requires BitVec.Intrinsics.forall_bool #256 (fun i -> i % 16 < 4 || vector i = 0))
       (fun _ -> Prims.l_True)
+
+include BitVec.Intrinsics {mm256_si256_from_two_si128 as mm256_si256_from_two_si128}
+
+val deserialize_10___deserialize_10_vec
+      (lower_coefficients0 upper_coefficients0: Libcrux_intrinsics.Avx2_extract.t_Vec128)
+    : Prims.Pure Libcrux_intrinsics.Avx2_extract.t_Vec256
+      Prims.l_True
+      (ensures
+        fun coefficients ->
+          let coefficients:Libcrux_intrinsics.Avx2_extract.t_Vec256 = coefficients in
+          forall (i: nat{i < 256}).
+            coefficients i =
+            (if i % 16 >= 10 then 0
+              else
+                let j = (i / 16) * 10 + i % 16 in
+                if i < 128 then lower_coefficients0 j else upper_coefficients0 (j - 32)))
+
+val deserialize_10_ (bytes: t_Slice u8)
+    : Prims.Pure Libcrux_intrinsics.Avx2_extract.t_Vec256
+      (requires Seq.length bytes == 20)
+      (ensures
+        fun result ->
+          let result:Libcrux_intrinsics.Avx2_extract.t_Vec256 = result in
+          forall (i: nat{i < 256}).
+            result i =
+            (if i % 16 >= 10
+              then 0
+              else
+                let j = (i / 16) * 10 + i % 16 in
+                bit_vec_of_int_t_array (bytes <: t_Array _ (sz 20)) 8 j))
+
+val deserialize_12___deserialize_12_vec
+      (lower_coefficients0 upper_coefficients0: Libcrux_intrinsics.Avx2_extract.t_Vec128)
+    : Prims.Pure Libcrux_intrinsics.Avx2_extract.t_Vec256
+      Prims.l_True
+      (ensures
+        fun coefficients ->
+          let coefficients:Libcrux_intrinsics.Avx2_extract.t_Vec256 = coefficients in
+          forall (i: nat{i < 256}).
+            coefficients i =
+            (if i % 16 >= 12 then 0
+             else let j = (i / 16) * 12 + i % 16 in
+                  if i < 128 then lower_coefficients0 j else upper_coefficients0 (j - 64)))
+
+val deserialize_12_ (bytes: t_Slice u8)
+    : Prims.Pure Libcrux_intrinsics.Avx2_extract.t_Vec256
+      (requires Seq.length bytes == 24)
+      (ensures
+        fun result ->
+          let result:Libcrux_intrinsics.Avx2_extract.t_Vec256 = result in
+          forall (i: nat{i < 256}).
+            result i =
+            (if i % 16 >= 12
+              then 0
+              else
+                let j = (i / 16) * 12 + i % 16 in
+                bit_vec_of_int_t_array (bytes <: t_Array _ (sz 24)) 8 j))
+
+val deserialize_5_ (bytes: t_Slice u8)
+    : Prims.Pure Libcrux_intrinsics.Avx2_extract.t_Vec256 Prims.l_True (fun _ -> Prims.l_True)
 
 val deserialize_11_ (bytes: t_Slice u8)
     : Prims.Pure Libcrux_intrinsics.Avx2_extract.t_Vec256 Prims.l_True (fun _ -> Prims.l_True)
