fstar-helpers/fstar-bitvec/BitVec.Utils.fst
@@ -13,6 +13,12 @@ let mk_list_32 #a (x0 x1 x2 x3 x4 x5 x6 x7 x8 x9 x10 x11 x12 x13 x14 x15 x16 x17
     assert_norm (List.Tot.length l == 32);
     l
 
+let mk_list_16 #a (x0 x1 x2 x3 x4 x5 x6 x7 x8 x9 x10 x11 x12 x13 x14 x15: a)
+  : (l:list a {List.Tot.length l == 16})
+  = let l = [x0;x1;x2;x3;x4;x5;x6;x7;x8;x9;x10;x11;x12;x13;x14;x15] in
+    assert_norm (List.Tot.length l == 16);
+    l
+
 let mk_list_8 #a (x0 x1 x2 x3 x4 x5 x6 x7: a)
   : (l:list a {List.Tot.length l == 8})
   = let l = [x0;x1;x2;x3;x4;x5;x6;x7] in
@@ -35,3 +41,19 @@ let rw_get_bit_shr #t #u (x: int_t t) (y: int_t u) (i: usize {v i < bits t})
                          then get_bit x (mk_int (bits t - 1))
                          else 0))
   = ()
+
+unfold type forall_sig (n: nat) = pred: ((i:nat{i < n}) -> bool)
+                              -> r: bool {r <==> (forall i. pred i)}
+
+let forall8: forall_sig 8 = fun pred -> pred 0 && pred 1 && pred 2 && pred 3
+                                  && pred 4 && pred 5 && pred 6 && pred 7
+
+#push-options "--z3rlimit 400"
+let forall16: forall_sig 16 = fun pred -> forall8 pred && forall8 (fun i -> pred (i + 8))
+let forall32: forall_sig 32 = fun pred -> forall16 pred && forall16 (fun i -> pred (i + 16))
+let forall64: forall_sig 64 = fun pred -> forall32 pred && forall32 (fun i -> pred (i + 32))
+let forall128: forall_sig 128 = fun pred -> forall64 pred && forall64 (fun i -> pred (i + 64))
+let forall256: forall_sig 256 = fun pred -> forall128 pred && forall128 (fun i -> pred (i + 128))
+#pop-options
+
+let forall_n (n:nat{n <= 256}): forall_sig n = fun pred -> forall256 (fun i -> if i < n then pred i else true)
