libcrux-intrinsics/proofs/fstar/extraction/Libcrux_intrinsics.Avx2_extract.fsti
@@ -67,28 +67,22 @@ val mm256_permute2x128_si256 (v_IMM8: i32) (a b: t_Vec256)
 val mm256_permute4x64_epi64 (v_CONTROL: i32) (vector: t_Vec256)
     : Prims.Pure t_Vec256 Prims.l_True (fun _ -> Prims.l_True)
 
-val mm256_permutevar8x32_epi32 (vector control: t_Vec256)
-    : Prims.Pure t_Vec256 Prims.l_True (fun _ -> Prims.l_True)
+include BitVec.Intrinsics {mm256_permutevar8x32_epi32}
 
 val mm256_set1_epi32 (constant: i32) : Prims.Pure t_Vec256 Prims.l_True (fun _ -> Prims.l_True)
 
 val mm256_set1_epi64x (a: i64) : Prims.Pure t_Vec256 Prims.l_True (fun _ -> Prims.l_True)
 
-val mm256_set_epi32 (input7 input6 input5 input4 input3 input2 input1 input0: i32)
-    : Prims.Pure t_Vec256 Prims.l_True (fun _ -> Prims.l_True)
+include BitVec.Intrinsics {mm256_set_epi32}
 
-val mm256_set_epi8
-      (byte31 byte30 byte29 byte28 byte27 byte26 byte25 byte24 byte23 byte22 byte21 byte20 byte19 byte18 byte17 byte16 byte15 byte14 byte13 byte12 byte11 byte10 byte9 byte8 byte7 byte6 byte5 byte4 byte3 byte2 byte1 byte0:
-          i8)
-    : Prims.Pure t_Vec256 Prims.l_True (fun _ -> Prims.l_True)
+include BitVec.Intrinsics {mm256_set_epi8}
 
 val mm256_setzero_si256: Prims.unit -> Prims.Pure t_Vec256 Prims.l_True (fun _ -> Prims.l_True)
 
 val mm256_shuffle_epi32 (v_CONTROL: i32) (vector: t_Vec256)
     : Prims.Pure t_Vec256 Prims.l_True (fun _ -> Prims.l_True)
 
-val mm256_shuffle_epi8 (vector control: t_Vec256)
-    : Prims.Pure t_Vec256 Prims.l_True (fun _ -> Prims.l_True)
+include BitVec.Intrinsics {mm256_shuffle_epi8}
 
 val mm256_slli_epi32 (v_SHIFT_BY: i32) (vector: t_Vec256)
     : Prims.Pure t_Vec256 Prims.l_True (fun _ -> Prims.l_True)
@@ -96,8 +90,7 @@ val mm256_slli_epi32 (v_SHIFT_BY: i32) (vector: t_Vec256)
 val mm256_slli_epi64 (v_LEFT: i32) (x: t_Vec256)
     : Prims.Pure t_Vec256 Prims.l_True (fun _ -> Prims.l_True)
 
-val mm256_sllv_epi32 (vector counts: t_Vec256)
-    : Prims.Pure t_Vec256 Prims.l_True (fun _ -> Prims.l_True)
+include BitVec.Intrinsics {mm256_sllv_epi32}
 
 val mm256_srai_epi16 (v_SHIFT_BY: i32) (vector: t_Vec256)
     : Prims.Pure t_Vec256
@@ -112,9 +105,6 @@ val mm256_srai_epi32 (v_SHIFT_BY: i32) (vector: t_Vec256)
     : Prims.Pure t_Vec256 Prims.l_True (fun _ -> Prims.l_True)
 
 val mm256_srli_epi32 (v_SHIFT_BY: i32) (vector: t_Vec256)
-    : Prims.Pure t_Vec256 Prims.l_True (fun _ -> Prims.l_True)
-
-val mm256_srli_epi64 (v_SHIFT_BY: i32) (vector: t_Vec256)
     : Prims.Pure t_Vec256 Prims.l_True (fun _ -> Prims.l_True)
 
 val mm256_storeu_si256_i16 (output: t_Slice i16) (vector: t_Vec256)
@@ -154,7 +144,7 @@ val mm_add_epi16 (lhs rhs: t_Vec128)
           vec128_as_i16x8 result ==
           Spec.Utils.map2 ( +. ) (vec128_as_i16x8 lhs) (vec128_as_i16x8 rhs))
 
-val mm_loadu_si128 (input: t_Slice u8) : Prims.Pure t_Vec128 Prims.l_True (fun _ -> Prims.l_True)
+include BitVec.Intrinsics {mm_loadu_si128}
 
 val mm_mulhi_epi16 (lhs rhs: t_Vec128)
     : Prims.Pure t_Vec128
@@ -184,13 +174,9 @@ val mm_set1_epi16 (constant: i16)
           let result:t_Vec128 = result in
           vec128_as_i16x8 result == Spec.Utils.create (sz 8) constant)
 
-val mm_set_epi8
-      (byte15 byte14 byte13 byte12 byte11 byte10 byte9 byte8 byte7 byte6 byte5 byte4 byte3 byte2 byte1 byte0:
-          u8)
-    : Prims.Pure t_Vec128 Prims.l_True (fun _ -> Prims.l_True)
+include BitVec.Intrinsics {mm_set_epi8}
 
-val mm_shuffle_epi8 (vector control: t_Vec128)
-    : Prims.Pure t_Vec128 Prims.l_True (fun _ -> Prims.l_True)
+include BitVec.Intrinsics {mm_shuffle_epi8}
 
 include BitVec.Intrinsics {mm_storeu_bytes_si128}
 
@@ -247,6 +233,8 @@ let lemma_mm256_set_epi16 v15 v14 v13 v12 v11 v10 v9 v8 v7 v6 v5 v4 v3 v2 v1 v0 
 include BitVec.Intrinsics {mm256_slli_epi16 as mm256_slli_epi16}
 
 include BitVec.Intrinsics {mm256_srli_epi16 as mm256_srli_epi16}
+
+include BitVec.Intrinsics {mm256_srli_epi64 as mm256_srli_epi64}
 
 include BitVec.Intrinsics {mm_movemask_epi8 as mm_movemask_epi8}
 
